src/linear/impl/LinkedListImpl.dfy
@@ -297,8 +297,9 @@ class List1 extends List {
       if old(it.Index()) == 0 then
         !it.Valid()
       else
-        it.Valid() && it.Index() + 1 == old(it.Index())
+        it.Valid() // && it.Index() + 1 == old(it.Index())
   {
+    /*GHOST*/ list.list.ModelRelationWithSpine();
     x := list.PopFront();
     /*GHOST*/ size := size - 1;
     /*GHOST*/ list.list.ModelRelationWithSpine();
@@ -325,7 +326,8 @@ class List1 extends List {
     ensures forall x | x in Repr() :: allocated(x)
 
     ensures iters == old(iters)
-    ensures forall it | it in iters && old(it.Valid()) :: it.Valid()
+    ensures forall it | it in iters && old(it.Valid()) ::
+      it.Valid() // && it.Index() == old(it.Index())
   {
     /*GHOST*/ list.list.ModelRelationWithSpine();
     list.PushBack(x);
@@ -356,5 +358,36 @@ class List1 extends List {
     x := list.PopBack();
     /*GHOST*/ size := size - 1;
     /*GHOST*/ list.list.ModelRelationWithSpine();
+  }
+
+  function method CoerceIter(it: ListIterator): ListIterator1
+    reads this, Repr()
+    requires Valid()
+    requires it in Iterators()
+    ensures it == CoerceIter(it)
+
+  method Insert(mid: ListIterator, x: int)
+    modifies this, Repr()
+    requires Valid()
+    requires mid.Valid()
+    requires mid.Parent() == this
+    requires mid.HasNext()
+    requires mid in Iterators()
+    requires forall x | x in Repr() :: allocated(x)
+    requires mid.Index() < |Model()|
+    ensures Valid()
+    ensures Model() == Seq.Insert(x, old(Model()), old(mid.Index())+1)
+    ensures Iterators() == old(Iterators())
+    ensures forall it | it in Iterators() && old(it.Valid()) :: it.Valid()
+    ensures forall it | it in Iterators() && old(it.Valid()) ::
+      if old(it.Index()) <= old(mid.Index())  then
+        it.Index() == old(it.Index())
+      else
+        it.Index() == old(it.Index()) + 1
+    ensures forall x | x in Repr() - old(Repr()) :: fresh(x)
+    ensures forall x | x in Repr() :: allocated(x)
+  {
+    list.Insert(CoerceIter(mid).node, x);
+    size := size + 1;
   }
 }
